erasure/theories/EInlineProjections.v
@@ -1,0 +1,891 @@
+(* Distributed under the terms of the MIT license. *)
+From Coq Require Import Utf8 Program.
+From MetaCoq.Template Require Import config utils Kernames.
+From MetaCoq.PCUIC Require Import PCUICAst PCUICAstUtils
+     PCUICReflect PCUICWeakeningEnvConv PCUICWeakeningEnvTyp
+     PCUICTyping PCUICInversion
+     PCUICSafeLemmata. (* for welltyped *)
+From MetaCoq.SafeChecker Require Import PCUICWfEnvImpl.
+From MetaCoq.Erasure Require Import EAst EAstUtils EDeps EExtends
+    ELiftSubst ECSubst EGlobalEnv EWellformed EWcbvEval Extract Prelim
+    EEnvMap EArities EProgram.
+
+Local Open Scope string_scope.
+Set Asymmetric Patterns.
+Import MCMonadNotation.
+
+From Equations Require Import Equations.
+Set Equations Transparent.
+Local Set Keyed Unification.
+Require Import ssreflect ssrbool.
+
+(** We assumes [Prop </= Type] and universes are checked correctly in the following. *)
+Local Existing Instance extraction_checker_flags.
+
+Ltac introdep := let H := fresh in intros H; depelim H.
+
+#[global]
+Hint Constructors eval : core.
+
+Section optimize.
+  Context (Σ : GlobalContextMap.t).
+
+  Fixpoint optimize (t : term) : term :=
+    match t with
+    | tRel i => tRel i
+    | tEvar ev args => tEvar ev (List.map optimize args)
+    | tLambda na M => tLambda na (optimize M)
+    | tApp u v => tApp (optimize u) (optimize v)
+    | tLetIn na b b' => tLetIn na (optimize b) (optimize b')
+    | tCase ind c brs => tCase ind (optimize c) (map (on_snd optimize) brs)
+    | tProj p c =>
+      match GlobalContextMap.lookup_constructor Σ p.1.1 0 with 
+      | Some (mdecl, idecl, cdecl) => 
+        tCase p.1 (optimize c) [(unfold cdecl.2 (fun n => nAnon), tRel (cdecl.2 - S p.2))]
+      | _ => tProj p (optimize c)
+      end
+    | tFix mfix idx =>
+      let mfix' := List.map (map_def optimize) mfix in
+      tFix mfix' idx
+    | tCoFix mfix idx =>
+      let mfix' := List.map (map_def optimize) mfix in
+      tCoFix mfix' idx
+    | tBox => t
+    | tVar _ => t
+    | tConst _ => t
+    | tConstruct _ _ => t
+    (* | tPrim _ => t *)
+    end.
+
+  Lemma optimize_mkApps f l : optimize (mkApps f l) = mkApps (optimize f) (map optimize l).
+  Proof.
+    induction l using rev_ind; simpl; auto.
+    now rewrite mkApps_app /= IHl map_app /= mkApps_app /=.
+  Qed.
+
+  Lemma map_repeat {A B} (f : A -> B) x n : map f (repeat x n) = repeat (f x) n.
+  Proof.
+    now induction n; simpl; auto; rewrite IHn.
+  Qed.
+  
+  Lemma map_optimize_repeat_box n : map optimize (repeat tBox n) = repeat tBox n.
+  Proof. by rewrite map_repeat. Qed.
+
+  Import ECSubst.
+
+  Lemma closed_optimize t k : closedn k t -> closedn k (optimize t).
+  Proof.
+    induction t in k |- * using EInduction.term_forall_list_ind; simpl; auto;
+    intros; try easy;
+    rewrite -> ?map_map_compose, ?compose_on_snd, ?compose_map_def, ?map_length;
+    unfold test_def in *;
+    simpl closed in *; try solve [simpl subst; simpl closed; f_equal; auto; rtoProp; solve_all]; try easy.
+    - move/andP: H => [] clt cll.
+      rewrite IHt //=. solve_all.
+    - destruct GlobalContextMap.lookup_constructor as [[[mdecl idecl] cdecl]|]; cbn; auto.
+      rewrite IHt //=; len. rewrite andb_true_r; apply Nat.ltb_lt. 
+      assert (cdecl.2 > 0). admit. lia.
+      lia.
+  Qed.
+ 
+  Lemma optimize_csubst a k b : 
+    closed a ->
+    optimize (ECSubst.csubst a k b) = ECSubst.csubst (optimize a) k (optimize b).
+  Proof.
+    induction b in k |- * using EInduction.term_forall_list_ind; simpl; auto;
+    intros cl; try easy; 
+    rewrite -> ?map_map_compose, ?compose_on_snd, ?compose_map_def, ?map_length;
+    unfold test_def in *;
+    simpl closed in *; try solve [simpl subst; simpl closed; f_equal; auto; rtoProp; solve_all]; try easy.
+    - destruct (k ?= n)%nat; auto.
+    - destruct GlobalContextMap.inductive_isprop_and_pars as [[[|] _]|] => /= //.
+      destruct l as [|[br n] [|l']] eqn:eql; simpl.
+      all:unfold on_snd; cbn.
+      * f_equal; auto.
+      * depelim X. simpl in *.
+        rewrite e //.
+        assert (#|br| = #|repeat tBox #|br| |). now rewrite repeat_length.
+        rewrite {2}H.
+        rewrite substl_csubst_comm //.
+        solve_all. eapply All_repeat => //.
+        now eapply closed_optimize.
+      * depelim X. depelim X.
+        f_equal; eauto.
+        unfold on_snd; cbn. f_equal; eauto.
+        f_equal; eauto.
+        f_equal; eauto. f_equal; eauto.
+        rewrite map_map_compose; solve_all.
+      * rewrite ?map_map_compose; f_equal; eauto; solve_all.
+      * rewrite ?map_map_compose; f_equal; eauto; solve_all.
+    - destruct GlobalContextMap.inductive_isprop_and_pars as [[[|] _]|]=> //;
+      now rewrite IHb.
+  Qed.
+
+  Lemma optimize_substl s t : 
+    forallb (closedn 0) s ->
+    optimize (substl s t) = substl (map optimize s) (optimize t).
+  Proof.
+    induction s in t |- *; simpl; auto.
+    move/andP => [] cla cls.
+    rewrite IHs //. f_equal.
+    now rewrite optimize_csubst.
+  Qed.
+
+  Lemma optimize_iota_red pars args br :
+    forallb (closedn 0) args ->
+    optimize (EGlobalEnv.iota_red pars args br) = EGlobalEnv.iota_red pars (map optimize args) (on_snd optimize br).
+  Proof.
+    intros cl.
+    unfold EGlobalEnv.iota_red.
+    rewrite optimize_substl //.
+    rewrite forallb_rev forallb_skipn //.
+    now rewrite map_rev map_skipn.
+  Qed.
+  
+  Lemma optimize_fix_subst mfix : EGlobalEnv.fix_subst (map (map_def optimize) mfix) = map optimize (EGlobalEnv.fix_subst mfix).
+  Proof.
+    unfold EGlobalEnv.fix_subst.
+    rewrite map_length.
+    generalize #|mfix|.
+    induction n; simpl; auto.
+    f_equal; auto.
+  Qed.
+
+  Lemma optimize_cofix_subst mfix : EGlobalEnv.cofix_subst (map (map_def optimize) mfix) = map optimize (EGlobalEnv.cofix_subst mfix).
+  Proof.
+    unfold EGlobalEnv.cofix_subst.
+    rewrite map_length.
+    generalize #|mfix|.
+    induction n; simpl; auto.
+    f_equal; auto.
+  Qed.
+
+  Lemma optimize_cunfold_fix mfix idx n f : 
+    forallb (closedn 0) (EGlobalEnv.fix_subst mfix) ->
+    cunfold_fix mfix idx = Some (n, f) ->
+    cunfold_fix (map (map_def optimize) mfix) idx = Some (n, optimize f).
+  Proof.
+    intros hfix.
+    unfold cunfold_fix.
+    rewrite nth_error_map.
+    destruct nth_error.
+    intros [= <- <-] => /=. f_equal.
+    now rewrite optimize_substl // optimize_fix_subst.
+    discriminate.
+  Qed.
+
+  Lemma optimize_cunfold_cofix mfix idx n f : 
+    forallb (closedn 0) (EGlobalEnv.cofix_subst mfix) ->
+    cunfold_cofix mfix idx = Some (n, f) ->
+    cunfold_cofix (map (map_def optimize) mfix) idx = Some (n, optimize f).
+  Proof.
+    intros hcofix.
+    unfold cunfold_cofix.
+    rewrite nth_error_map.
+    destruct nth_error.
+    intros [= <- <-] => /=. f_equal.
+    now rewrite optimize_substl // optimize_cofix_subst.
+    discriminate.
+  Qed.
+
+  Lemma optimize_nth {n l d} : 
+    optimize (nth n l d) = nth n (map optimize l) (optimize d).
+  Proof.
+    induction l in n |- *; destruct n; simpl; auto.
+  Qed.
+
+End optimize.
+
+Lemma is_box_inv b : is_box b -> ∑ args, b = mkApps tBox args.
+Proof.
+  unfold is_box, EAstUtils.head.
+  destruct decompose_app eqn:da.
+  simpl. destruct t => //.
+  eapply decompose_app_inv in da. subst.
+  eexists; eauto.
+Qed.
+
+Lemma eval_is_box {wfl:WcbvFlags} Σ t u : Σ ⊢ t ▷ u -> is_box t -> u = EAst.tBox.
+Proof.
+  intros ev; induction ev => //.
+  - rewrite is_box_tApp.
+    intros isb. intuition congruence.
+  - rewrite is_box_tApp. move/IHev1 => ?; solve_discr.
+  - rewrite is_box_tApp. move/IHev1 => ?; solve_discr.
+  - rewrite is_box_tApp. move/IHev1 => ?. subst => //.
+  - rewrite is_box_tApp. move/IHev1 => ?. subst. solve_discr.
+  - rewrite is_box_tApp. move/IHev1 => ?. subst. cbn in i.
+    destruct EWcbvEval.with_guarded_fix => //.
+  - destruct t => //.
+Qed. 
+
+Lemma isType_tSort {cf:checker_flags} {Σ : global_env_ext} {Γ l A} {wfΣ : wf Σ} : Σ ;;; Γ |- tSort (Universe.make l) : A -> isType Σ Γ (tSort (Universe.make l)).
+Proof.
+  intros HT.
+  eapply inversion_Sort in HT as [l' [wfΓ Hs]]; auto.
+  eexists; econstructor; eauto.
+Qed.
+
+Lemma isType_it_mkProd {cf:checker_flags} {Σ : global_env_ext} {Γ na dom codom A} {wfΣ : wf Σ} :   
+  Σ ;;; Γ |- tProd na dom codom : A -> 
+  isType Σ Γ (tProd na dom codom).
+Proof.
+  intros HT.
+  eapply inversion_Prod in HT as (? & ? & ? & ? & ?); auto.
+  eexists; econstructor; eauto.
+Qed.
+
+Definition optimize_constant_decl Σ cb := 
+  {| cst_body := option_map (optimize Σ) cb.(cst_body) |}.
+  
+Definition optimize_decl Σ d :=
+  match d with
+  | ConstantDecl cb => ConstantDecl (optimize_constant_decl Σ cb)
+  | InductiveDecl idecl => d
+  end.
+
+Definition optimize_env Σ := 
+  map (on_snd (optimize_decl Σ)) Σ.(GlobalContextMap.global_decls).
+  
+Import EnvMap.
+
+Program Fixpoint optimize_env' Σ : EnvMap.fresh_globals Σ -> global_context :=
+  match Σ with
+  | [] => fun _ => []
+  | hd :: tl => fun HΣ =>
+    let Σg := GlobalContextMap.make tl (fresh_globals_cons_inv HΣ) in 
+    on_snd (optimize_decl Σg) hd :: optimize_env' tl (fresh_globals_cons_inv HΣ) 
+  end.
+
+Import EGlobalEnv EExtends.
+
+(* Lemma extends_is_propositional {Σ Σ'} : 
+  wf_glob Σ' -> extends Σ Σ' ->
+  forall ind, 
+  match inductive_isprop_and_pars Σ ind with
+  | Some b => inductive_isprop_and_pars Σ' ind = Some b
+  | None => inductive_isprop_and_pars Σ' ind = None
+  end.
+Proof.
+  intros wf ex ind.
+  rewrite /inductive_isprop_and_pars.
+  destruct lookup_env eqn:lookup => //.
+  now rewrite (extends_lookup wf ex lookup).
+
+Qed. *)
+
+Lemma extends_inductive_isprop_and_pars {efl : EEnvFlags} {Σ Σ' ind} : extends Σ Σ' -> wf_glob Σ' ->
+  isSome (lookup_inductive Σ ind) -> 
+  inductive_isprop_and_pars Σ ind = inductive_isprop_and_pars Σ' ind.
+Proof.
+  intros ext wf; cbn.
+  unfold inductive_isprop_and_pars.
+  destruct lookup_env as [[]|] eqn:hl => //.
+  rewrite (extends_lookup wf ext hl).
+  destruct nth_error => //.
+Qed.
+
+Lemma wellformed_optimize_extends {wfl: EEnvFlags} {Σ : GlobalContextMap.t} t : 
+  forall n, EWellformed.wellformed Σ n t ->
+  forall {Σ' : GlobalContextMap.t}, extends Σ Σ' -> wf_glob Σ' ->
+  optimize Σ t = optimize Σ' t.
+Proof.
+  induction t using EInduction.term_forall_list_ind; cbn -[lookup_constant lookup_inductive
+    GlobalContextMap.inductive_isprop_and_pars]; intros => //.
+  all:unfold wf_fix_gen in *; rtoProp; intuition auto.  
+  all:f_equal; eauto; solve_all.
+  - rewrite !GlobalContextMap.inductive_isprop_and_pars_spec.
+    assert (map (on_snd (optimize Σ)) l = map (on_snd (optimize Σ')) l) as -> by solve_all.
+    rewrite (extends_inductive_isprop_and_pars H0 H1 H2).
+    destruct inductive_isprop_and_pars as [[[]]|].
+    destruct map => //. f_equal; eauto.
+    destruct l0 => //. destruct p0 => //. f_equal; eauto.
+    all:f_equal; eauto; solve_all.
+  - rewrite !GlobalContextMap.inductive_isprop_and_pars_spec.
+    rewrite (extends_inductive_isprop_and_pars H0 H1 H3).
+    destruct inductive_isprop_and_pars as [[[]]|] => //.
+    all:f_equal; eauto.
+Qed.
+
+Lemma wellformed_optimize_decl_extends {wfl: EEnvFlags} {Σ : GlobalContextMap.t} t : 
+  wf_global_decl Σ t ->
+  forall {Σ' : GlobalContextMap.t}, extends Σ Σ' -> wf_glob Σ' ->
+  optimize_decl Σ t = optimize_decl Σ' t.
+Proof.
+  destruct t => /= //.
+  intros wf Σ' ext wf'. f_equal. unfold optimize_constant_decl. f_equal.
+  destruct (cst_body c) => /= //. f_equal.
+  now eapply wellformed_optimize_extends.
+Qed.
+
+Lemma lookup_env_optimize_env_Some {efl : EEnvFlags} {Σ : GlobalContextMap.t} kn d : 
+  wf_glob Σ ->
+  GlobalContextMap.lookup_env Σ kn = Some d ->
+  ∑ Σ' : GlobalContextMap.t, 
+    [× extends Σ' Σ, wf_global_decl Σ' d &
+      lookup_env (optimize_env Σ) kn = Some (optimize_decl Σ' d)].
+Proof.
+  rewrite GlobalContextMap.lookup_env_spec.
+  destruct Σ as [Σ map repr wf].
+  induction Σ in map, repr, wf |- *; simpl; auto => //.
+  intros wfg.
+  case: eqb_specT => //.
+  - intros ->. cbn. intros [= <-].
+    exists (GlobalContextMap.make Σ (fresh_globals_cons_inv wf)). split.
+    now eexists [_].
+    cbn. now depelim wfg.
+    f_equal. symmetry. eapply wellformed_optimize_decl_extends. cbn. now depelim wfg.
+    cbn. now exists [a]. now cbn.
+  - intros _. 
+    set (Σ' := GlobalContextMap.make Σ (fresh_globals_cons_inv wf)).
+    specialize (IHΣ (GlobalContextMap.map Σ') (GlobalContextMap.repr Σ') (GlobalContextMap.wf Σ')).
+    cbn in IHΣ. forward IHΣ. now depelim wfg.
+    intros hl. specialize (IHΣ hl) as [Σ'' [ext wfgd hl']].
+    exists Σ''. split => //.
+    * destruct ext as [? ->].
+      now exists (a :: x).
+    * rewrite -hl'. f_equal.
+      clear -wfg.
+      eapply map_ext_in => kn hin. unfold on_snd. f_equal.
+      symmetry. eapply wellformed_optimize_decl_extends => //. cbn.
+      eapply lookup_env_In in hin. 2:now depelim wfg.
+      depelim wfg. eapply lookup_env_wellformed; tea.
+      cbn. now exists [a].
+Qed.
+
+Lemma lookup_env_map_snd Σ f kn : lookup_env (List.map (on_snd f) Σ) kn = option_map f (lookup_env Σ kn).
+Proof.
+  induction Σ; cbn; auto.
+  case: eqb_spec => //.
+Qed.
+
+Lemma lookup_env_optimize_env_None {efl : EEnvFlags} {Σ : GlobalContextMap.t} kn : 
+  GlobalContextMap.lookup_env Σ kn = None ->
+  lookup_env (optimize_env Σ) kn = None.
+Proof.
+  rewrite GlobalContextMap.lookup_env_spec.
+  destruct Σ as [Σ map repr wf].
+  cbn. intros hl. rewrite lookup_env_map_snd hl //.
+Qed.
+
+Lemma lookup_env_optimize {efl : EEnvFlags} {Σ : GlobalContextMap.t} kn : 
+  wf_glob Σ ->
+  lookup_env (optimize_env Σ) kn = option_map (optimize_decl Σ) (lookup_env Σ kn).
+Proof.
+  intros wf.
+  rewrite -GlobalContextMap.lookup_env_spec.
+  destruct (GlobalContextMap.lookup_env Σ kn) eqn:hl.
+  - eapply lookup_env_optimize_env_Some in hl as [Σ' [ext wf' hl']] => /=.
+    rewrite hl'. f_equal.
+    eapply wellformed_optimize_decl_extends; eauto. auto.
+    
+  - cbn. now eapply lookup_env_optimize_env_None in hl. 
+Qed.
+
+Lemma is_propositional_optimize {efl : EEnvFlags} {Σ : GlobalContextMap.t} ind : 
+  wf_glob Σ ->
+  inductive_isprop_and_pars Σ ind = inductive_isprop_and_pars (optimize_env Σ) ind.
+Proof.
+  rewrite /inductive_isprop_and_pars => wf.
+  rewrite /lookup_inductive /lookup_minductive.
+  rewrite (lookup_env_optimize (inductive_mind ind) wf).
+  rewrite /GlobalContextMap.inductive_isprop_and_pars /GlobalContextMap.lookup_inductive
+    /GlobalContextMap.lookup_minductive.  
+  destruct lookup_env as [[decl|]|] => //.
+Qed.
+
+Lemma is_propositional_cstr_optimize {efl : EEnvFlags} {Σ : GlobalContextMap.t} ind c : 
+  wf_glob Σ ->
+  constructor_isprop_pars_decl Σ ind c = constructor_isprop_pars_decl (optimize_env Σ) ind c.
+Proof.
+  rewrite /constructor_isprop_pars_decl => wf.
+  rewrite /lookup_constructor /lookup_inductive /lookup_minductive.
+  rewrite (lookup_env_optimize (inductive_mind ind) wf).
+  rewrite /GlobalContextMap.inductive_isprop_and_pars /GlobalContextMap.lookup_inductive
+    /GlobalContextMap.lookup_minductive.  
+  destruct lookup_env as [[decl|]|] => //.
+Qed.
+
+
+Lemma closed_iota_red pars c args brs br :
+  forallb (closedn 0) args ->
+  nth_error brs c = Some br ->
+  #|skipn pars args| = #|br.1| ->
+  closedn #|br.1| br.2 ->
+  closed (iota_red pars args br).
+Proof.
+  intros clargs hnth hskip clbr.
+  rewrite /iota_red.
+  eapply ECSubst.closed_substl => //.
+  now rewrite forallb_rev forallb_skipn.
+  now rewrite List.rev_length hskip Nat.add_0_r.
+Qed.
+
+Definition disable_prop_cases fl := {| with_prop_case := false; with_guarded_fix := fl.(@with_guarded_fix) |}.
+
+Lemma isFix_mkApps t l : isFix (mkApps t l) = isFix t && match l with [] => true | _ => false end.
+Proof.
+  induction l using rev_ind; cbn.
+  - now rewrite andb_true_r.
+  - rewrite mkApps_app /=. now destruct l => /= //; rewrite andb_false_r.
+Qed.
+
+Lemma lookup_constructor_optimize {efl : EEnvFlags} {Σ : GlobalContextMap.t} {ind c} :
+  wf_glob Σ ->
+  lookup_constructor Σ ind c = lookup_constructor (optimize_env Σ) ind c.
+Proof.
+  intros wfΣ. rewrite /lookup_constructor /lookup_inductive /lookup_minductive.
+  rewrite lookup_env_optimize // /=. destruct lookup_env => // /=.
+  destruct g => //.
+Qed.
+
+Lemma constructor_isprop_pars_decl_inductive {Σ ind c} {prop pars cdecl} :
+  constructor_isprop_pars_decl Σ ind c = Some (prop, pars, cdecl)  -> 
+  inductive_isprop_and_pars Σ ind = Some (prop, pars).
+Proof.
+  rewrite /constructor_isprop_pars_decl /inductive_isprop_and_pars /lookup_constructor.
+  destruct lookup_inductive as [[mdecl idecl]|]=> /= //.
+  destruct nth_error => //. congruence.
+Qed.
+
+Lemma optimize_correct {efl : EEnvFlags} {fl} {Σ : GlobalContextMap.t} t v :
+  wf_glob Σ ->
+  closed_env Σ ->
+  @Ee.eval fl Σ t v ->
+  closed t ->
+  @Ee.eval (disable_prop_cases fl) (optimize_env Σ) (optimize Σ t) (optimize Σ v).
+Proof.
+  intros wfΣ clΣ ev.
+  induction ev; simpl in *.
+
+  - move/andP => [] cla clt. econstructor; eauto.
+  - move/andP => [] clf cla.
+    eapply eval_closed in ev2; tea.
+    eapply eval_closed in ev1; tea.
+    econstructor; eauto.
+    rewrite optimize_csubst // in IHev3.
+    apply IHev3. eapply closed_csubst => //.
+
+  - move/andP => [] clb0 clb1. rewrite optimize_csubst in IHev2.
+    now eapply eval_closed in ev1.
+    econstructor; eauto. eapply IHev2, closed_csubst => //.
+    now eapply eval_closed in ev1.
+
+  - move/andP => [] cld clbrs. rewrite optimize_mkApps in IHev1.
+    have := (eval_closed _ clΣ _ _ cld ev1); rewrite closedn_mkApps => /andP[] _ clargs.
+    rewrite optimize_iota_red in IHev2.
+    eapply eval_closed in ev1 => //.
+    rewrite GlobalContextMap.inductive_isprop_and_pars_spec.
+    rewrite (constructor_isprop_pars_decl_inductive e).
+    eapply eval_iota; eauto. tea.
+    now rewrite -is_propositional_cstr_optimize.
+    rewrite nth_error_map e0 //. now len. cbn.
+    rewrite -e2. rewrite !skipn_length map_length //.
+    eapply IHev2.
+    eapply closed_iota_red => //; tea.
+    eapply nth_error_forallb in clbrs; tea. cbn in clbrs.
+    now rewrite Nat.add_0_r in clbrs.
+  
+  - move/andP => [] cld clbrs.
+    rewrite GlobalContextMap.inductive_isprop_and_pars_spec.
+    rewrite e e0 /=.
+    subst brs. cbn in clbrs. rewrite Nat.add_0_r andb_true_r in clbrs.
+    rewrite optimize_substl in IHev2. 
+    eapply All_forallb, All_repeat => //.
+    rewrite map_optimize_repeat_box in IHev2.
+    apply IHev2.
+    eapply closed_substl.
+    eapply All_forallb, All_repeat => //.
+    now rewrite repeat_length Nat.add_0_r.
+
+  - move/andP => [] clf cla. rewrite optimize_mkApps in IHev1.
+    simpl in *.
+    eapply eval_closed in ev1 => //.
+    rewrite closedn_mkApps in ev1.
+    move: ev1 => /andP [] clfix clargs.
+    eapply Ee.eval_fix; eauto.
+    rewrite map_length.
+    eapply optimize_cunfold_fix; tea.
+    eapply closed_fix_subst. tea.
+    rewrite optimize_mkApps in IHev3. apply IHev3.
+    rewrite closedn_mkApps clargs.
+    eapply eval_closed in ev2; tas. rewrite ev2 /= !andb_true_r.
+    eapply closed_cunfold_fix; tea.
+
+  - move/andP => [] clf cla.
+    eapply eval_closed in ev1 => //.
+    rewrite closedn_mkApps in ev1.
+    move: ev1 => /andP [] clfix clargs.
+    eapply eval_closed in ev2; tas.
+    rewrite optimize_mkApps in IHev1 |- *.
+    simpl in *. eapply Ee.eval_fix_value. auto. auto. auto.
+    eapply optimize_cunfold_fix; eauto.
+    eapply closed_fix_subst => //.
+    now rewrite map_length. 
+  
+  - move/andP => [] clf cla.
+    eapply eval_closed in ev1 => //.
+    eapply eval_closed in ev2; tas.
+    simpl in *. eapply Ee.eval_fix'. auto. auto.
+    eapply optimize_cunfold_fix; eauto.
+    eapply closed_fix_subst => //.
+    eapply IHev2; tea. eapply IHev3.
+    apply/andP; split => //.
+    eapply closed_cunfold_fix; tea.
+
+  - move/andP => [] cd clbrs. specialize (IHev1 cd).
+    rewrite closedn_mkApps in IHev2.
+    move: (eval_closed _ clΣ _ _ cd ev1).
+    rewrite closedn_mkApps.
+    move/andP => [] clfix clargs.
+    forward IHev2.
+    { rewrite clargs clbrs !andb_true_r.
+      eapply closed_cunfold_cofix; tea. }
+    rewrite -> optimize_mkApps in IHev1, IHev2. simpl.
+    rewrite GlobalContextMap.inductive_isprop_and_pars_spec in IHev2 |- *.
+    destruct EGlobalEnv.inductive_isprop_and_pars as [[[] pars]|] eqn:isp => //.
+    destruct brs as [|[a b] []]; simpl in *; auto.
+    simpl in IHev1.
+    eapply Ee.eval_cofix_case. tea.
+    apply optimize_cunfold_cofix; tea. eapply closed_cofix_subst; tea.
+    apply IHev2.
+    eapply Ee.eval_cofix_case; tea.
+    apply optimize_cunfold_cofix; tea. eapply closed_cofix_subst; tea.
+    simpl in *.
+    eapply Ee.eval_cofix_case; tea.
+    apply optimize_cunfold_cofix; tea. eapply closed_cofix_subst; tea.
+    eapply Ee.eval_cofix_case; tea.
+    apply optimize_cunfold_cofix; tea. eapply closed_cofix_subst; tea.
+    
+  - intros cd. specialize (IHev1 cd).
+    move: (eval_closed _ clΣ _ _ cd ev1).
+    rewrite closedn_mkApps; move/andP => [] clfix clargs. forward IHev2.
+    { rewrite closedn_mkApps clargs andb_true_r. eapply closed_cunfold_cofix; tea. }
+    rewrite GlobalContextMap.inductive_isprop_and_pars_spec in IHev2 |- *.
+    destruct EGlobalEnv.inductive_isprop_and_pars as [[[] pars]|] eqn:isp; auto.
+    rewrite -> optimize_mkApps in IHev1, IHev2. simpl in *.
+    econstructor; eauto.
+    apply optimize_cunfold_cofix; tea. eapply closed_cofix_subst; tea.
+    rewrite -> optimize_mkApps in IHev1, IHev2. simpl in *.
+    econstructor; eauto.
+    apply optimize_cunfold_cofix; tea. eapply closed_cofix_subst; tea.
+  
+  - rewrite /declared_constant in isdecl.
+    move: (lookup_env_optimize c wfΣ).
+    rewrite isdecl /= //.
+    intros hl.
+    econstructor; tea. cbn. rewrite e //.
+    apply IHev.
+    eapply lookup_env_closed in clΣ; tea.
+    move: clΣ. rewrite /closed_decl e //.
+  
+  - move=> cld.
+    eapply eval_closed in ev1; tea.
+    move: ev1; rewrite closedn_mkApps /= => clargs.
+    rewrite GlobalContextMap.inductive_isprop_and_pars_spec.
+    rewrite (constructor_isprop_pars_decl_inductive e).
+    rewrite optimize_mkApps in IHev1.
+    specialize (IHev1 cld).
+    eapply Ee.eval_proj; tea.
+    now rewrite -is_propositional_cstr_optimize.
+    now len. rewrite nth_error_map e1 //.
+    eapply IHev2.
+    eapply nth_error_forallb in e1; tea.
+
+  - rewrite GlobalContextMap.inductive_isprop_and_pars_spec.
+    now rewrite e.
+
+  - move/andP=> [] clf cla.
+    rewrite optimize_mkApps.
+    eapply eval_construct; tea.
+    rewrite -lookup_constructor_optimize //. exact e.
+    rewrite optimize_mkApps in IHev1. now eapply IHev1.
+    now len.
+    now eapply IHev2.
+
+  - move/andP => [] clf cla.
+    specialize (IHev1 clf). specialize (IHev2 cla).
+    eapply Ee.eval_app_cong; eauto.
+    eapply Ee.eval_to_value in ev1.
+    destruct ev1; simpl in *; eauto.
+    * destruct t => //; rewrite optimize_mkApps /=.
+    * destruct with_guarded_fix.
+      + move: i. 
+        rewrite !negb_or.
+        rewrite optimize_mkApps !isFixApp_mkApps !isConstructApp_mkApps.
+        destruct args using rev_case => // /=. rewrite map_app !mkApps_app /= //.
+        rewrite !andb_true_r.
+        rtoProp; intuition auto.
+        destruct v => /= //. 
+        destruct v => /= //.
+      + move: i. 
+        rewrite !negb_or.
+        rewrite optimize_mkApps !isConstructApp_mkApps.
+        destruct args using rev_case => // /=. rewrite map_app !mkApps_app /= //.
+        destruct v => /= //. 
+  - destruct t => //.
+    all:constructor; eauto.
+Qed.
+
+(* 
+Lemma optimize_extends Σ Σ' : 
+  wf_glob Σ' ->
+  extends Σ Σ' ->
+  forall t b, optimize Σ t = b -> optimize Σ' t = b.
+Proof.
+  intros wf ext.
+  induction t using EInduction.term_forall_list_ind; cbn => //.
+  all:try solve [f_equal; solve_all].
+  destruct inductive_isp
+  rewrite (extends_is_propositional wf ext).
+ *)
+
+From MetaCoq.Erasure Require Import EEtaExpanded.
+
+Lemma isLambda_optimize Σ t : isLambda t -> isLambda (optimize Σ t).
+Proof. destruct t => //. Qed.
+Lemma isBox_optimize Σ t : isBox t -> isBox (optimize Σ t).
+Proof. destruct t => //. Qed.
+
+Lemma optimize_expanded {Σ : GlobalContextMap.t} t : expanded Σ t -> expanded Σ (optimize Σ t).
+Proof.
+  induction 1 using expanded_ind.
+  all:try solve[constructor; eauto; solve_all].
+  all:rewrite ?optimize_mkApps.
+  - eapply expanded_mkApps_expanded => //. solve_all.
+  - cbn -[GlobalContextMap.inductive_isprop_and_pars].
+    rewrite GlobalContextMap.inductive_isprop_and_pars_spec.
+    destruct inductive_isprop_and_pars as [[[|] _]|] => /= //.
+    2-3:constructor; eauto; solve_all.
+    destruct branches eqn:heq.
+    constructor; eauto; solve_all. cbn.
+    destruct l => /=.
+    eapply isEtaExp_expanded.
+    eapply isEtaExp_substl. eapply forallb_repeat => //.
+    destruct branches as [|[]]; cbn in heq; noconf heq.
+    cbn -[isEtaExp] in *. depelim H1. cbn in H1.
+    now eapply expanded_isEtaExp.
+    constructor; eauto; solve_all.
+    depelim H1. depelim H1. do 2 (constructor; intuition auto).
+    solve_all.
+  - cbn -[GlobalContextMap.inductive_isprop_and_pars].
+    rewrite GlobalContextMap.inductive_isprop_and_pars_spec.
+    destruct inductive_isprop_and_pars as [[[|] _]|] => /= //.
+    constructor. all:constructor; auto.
+  - cbn. eapply expanded_tFix. solve_all.
+    rewrite isLambda_optimize //.
+  - eapply expanded_tConstruct_app; tea.
+    now len. solve_all.
+Qed.
+
+Lemma optimize_expanded_irrel {efl : EEnvFlags} {Σ : GlobalContextMap.t} t : wf_glob Σ -> expanded Σ t -> expanded (optimize_env Σ) t.
+Proof.
+  intros wf; induction 1 using expanded_ind.
+  all:try solve[constructor; eauto; solve_all].
+  eapply expanded_tConstruct_app.
+  destruct H as [[H ?] ?].
+  split => //. split => //. red.
+  red in H. rewrite lookup_env_optimize // /= H //. 1-2:eauto. auto. solve_all. 
+Qed.
+
+Lemma optimize_expanded_decl {Σ : GlobalContextMap.t} t : expanded_decl Σ t -> expanded_decl Σ (optimize_decl Σ t).
+Proof.
+  destruct t as [[[]]|] => /= //.
+  unfold expanded_constant_decl => /=.
+  apply optimize_expanded.
+Qed.
+
+Lemma optimize_expanded_decl_irrel {efl : EEnvFlags} {Σ : GlobalContextMap.t} t : wf_glob Σ -> expanded_decl Σ t -> expanded_decl (optimize_env Σ) t.
+Proof.
+  destruct t as [[[]]|] => /= //.
+  unfold expanded_constant_decl => /=.
+  apply optimize_expanded_irrel.
+Qed.
+
+Lemma optimize_env_extends' {efl : EEnvFlags} {Σ Σ' : GlobalContextMap.t} : 
+  extends Σ Σ' ->
+  wf_glob Σ' -> 
+  List.map (on_snd (optimize_decl Σ)) Σ.(GlobalContextMap.global_decls) =
+  List.map (on_snd (optimize_decl Σ')) Σ.(GlobalContextMap.global_decls).
+Proof.
+  intros ext.
+  destruct Σ as [Σ map repr wf]; cbn in *.
+  move=> wfΣ.
+  assert (extends Σ Σ); auto. now exists [].
+  assert (wf_glob Σ).
+  { eapply extends_wf_glob. exact ext. tea. }
+  revert H H0.
+  generalize Σ at 1 3 5 6. intros Σ''.
+  induction Σ'' => //. cbn.
+  intros hin wfg. depelim wfg.
+  f_equal.
+  2:{ eapply IHΣ'' => //. destruct hin. exists (x ++ [(kn, d)]). rewrite -app_assoc /= //. }
+  unfold on_snd. cbn. f_equal.
+  eapply wellformed_optimize_decl_extends => //. cbn.
+  eapply extends_wf_global_decl. 3:tea.
+  eapply extends_wf_glob; tea.
+  destruct hin. exists (x ++ [(kn, d)]). rewrite -app_assoc /= //.
+Qed.
+
+Lemma optimize_env_eq {efl : EEnvFlags} (Σ : GlobalContextMap.t) : wf_glob Σ -> optimize_env Σ = optimize_env' Σ.(GlobalContextMap.global_decls) Σ.(GlobalContextMap.wf).
+Proof.
+  intros wf.
+  unfold optimize_env.
+  destruct Σ; cbn. cbn in wf.
+  induction global_decls in map, repr, wf0, wf |- * => //.
+  cbn. f_equal.
+  destruct a as [kn d]; unfold on_snd; cbn. f_equal. symmetry.
+  eapply wellformed_optimize_decl_extends => //. cbn. now depelim wf. cbn. now exists [(kn, d)]. cbn.
+  set (Σg' := GlobalContextMap.make global_decls (fresh_globals_cons_inv wf0)).
+  erewrite <- (IHglobal_decls (GlobalContextMap.map Σg') (GlobalContextMap.repr Σg')).
+  2:now depelim wf.
+  set (Σg := {| GlobalContextMap.global_decls := _ :: _ |}).
+  symmetry. eapply (optimize_env_extends' (Σ := Σg') (Σ' := Σg)) => //.
+  cbn. now exists [a].
+Qed.
+
+Lemma optimize_env_expanded {efl : EEnvFlags} {Σ : GlobalContextMap.t} :
+  wf_glob Σ -> expanded_global_env Σ -> expanded_global_env (optimize_env Σ).
+Proof.
+  unfold expanded_global_env; move=> wfg.
+  rewrite optimize_env_eq //.
+  destruct Σ as [Σ map repr wf]. cbn in *.
+  clear map repr.
+  induction 1; cbn; constructor; auto.
+  cbn in IHexpanded_global_declarations.
+  unshelve eapply IHexpanded_global_declarations. now depelim wfg. cbn. 
+  set (Σ' := GlobalContextMap.make _ _).
+  rewrite -(optimize_env_eq Σ'). cbn. now depelim wfg.
+  eapply (optimize_expanded_decl_irrel (Σ := Σ')). now depelim wfg.
+  now unshelve eapply (optimize_expanded_decl (Σ:=Σ')).
+Qed.
+
+Lemma optimize_wellformed {efl : EEnvFlags} {Σ : GlobalContextMap.t} n t :
+  has_tBox -> has_tRel ->
+  wf_glob Σ -> EWellformed.wellformed Σ n t -> EWellformed.wellformed Σ n (optimize Σ t).
+Proof.
+  intros wfΣ hbox hrel.
+  induction t in n |- * using EInduction.term_forall_list_ind => //.
+  all:try solve [cbn; rtoProp; intuition auto; solve_all].
+  - cbn -[GlobalContextMap.inductive_isprop_and_pars lookup_inductive]. move/and3P => [] hasc /andP[]hs ht hbrs.
+    destruct GlobalContextMap.inductive_isprop_and_pars as [[[|] _]|] => /= //.
+    destruct l as [|[br n'] [|l']] eqn:eql; simpl.
+    all:rewrite ?hasc ?hs /= ?andb_true_r.
+    rewrite IHt //.
+    depelim X. cbn in hbrs.
+    rewrite andb_true_r in hbrs.
+    specialize (i _ hbrs).
+    eapply wellformed_substl => //. solve_all. eapply All_repeat => //.
+    now rewrite repeat_length.
+    cbn in hbrs; rtoProp; solve_all. depelim X; depelim X. solve_all.
+    do 2 depelim X. solve_all.
+    do 2 depelim X. solve_all.
+    rtoProp; solve_all. solve_all.
+    rtoProp; solve_all. solve_all.
+  - cbn -[GlobalContextMap.inductive_isprop_and_pars lookup_inductive]. move/andP => [] /andP[]hasc hs ht.
+    destruct GlobalContextMap.inductive_isprop_and_pars as [[[|] _]|] => /= //.
+    all:rewrite hasc hs /=; eauto.
+  - cbn. unfold wf_fix; rtoProp; intuition auto; solve_all. now len.
+    unfold test_def in *. len. eauto.
+  - cbn. unfold wf_fix; rtoProp; intuition auto; solve_all. now len.
+    unfold test_def in *. len. eauto.
+Qed.
+
+Import EWellformed.
+
+Lemma optimize_wellformed_irrel {efl : EEnvFlags} {Σ : GlobalContextMap.t} t :
+  wf_glob Σ ->
+  forall n, wellformed Σ n t -> wellformed (optimize_env Σ) n t.
+Proof.
+  intros wfΣ. induction t using EInduction.term_forall_list_ind; cbn => //.
+  all:try solve [intros; unfold wf_fix_gen in *; rtoProp; intuition eauto; solve_all].
+  - rewrite lookup_env_optimize //.
+    destruct lookup_env eqn:hl => // /=.
+    destruct g eqn:hg => /= //. subst g.
+    destruct (cst_body c) => //.
+  - rewrite lookup_env_optimize //.
+    destruct lookup_env eqn:hl => // /=.
+    destruct g eqn:hg => /= //. 
+  - rewrite lookup_env_optimize //.
+    destruct lookup_env eqn:hl => // /=.
+    destruct g eqn:hg => /= //. subst g.
+    destruct nth_error => /= //.
+    intros; rtoProp; intuition auto; solve_all.
+  - rewrite lookup_env_optimize //.
+    destruct lookup_env eqn:hl => // /=.
+    destruct g eqn:hg => /= //.
+    rewrite andb_false_r => //.
+    destruct nth_error => /= //.
+    all:intros; rtoProp; intuition auto; solve_all.
+Qed.
+
+Lemma optimize_wellformed_decl_irrel {efl : EEnvFlags} {Σ : GlobalContextMap.t} d :
+  wf_glob Σ ->
+  wf_global_decl Σ d -> wf_global_decl (optimize_env Σ) d.
+Proof.
+  intros wf; destruct d => /= //.
+  destruct (cst_body c) => /= //.
+  now eapply optimize_wellformed_irrel.
+Qed.
+
+Lemma optimize_decl_wf {efl : EEnvFlags} {Σ : GlobalContextMap.t} :
+  has_tBox -> has_tRel -> wf_glob Σ -> 
+  forall d, wf_global_decl Σ d -> wf_global_decl (optimize_env Σ) (optimize_decl Σ d).
+Proof.
+  intros hasb hasr wf d.
+  intros hd.
+  eapply optimize_wellformed_decl_irrel; tea.
+  move: hd.
+  destruct d => /= //.
+  destruct (cst_body c) => /= //.
+  now eapply optimize_wellformed => //.
+Qed.
+
+Lemma fresh_global_optimize_env {Σ : GlobalContextMap.t} kn : 
+  fresh_global kn Σ ->
+  fresh_global kn (optimize_env Σ).
+Proof.
+  destruct Σ as [Σ map repr wf]; cbn in *.
+  induction 1; cbn; constructor; auto.
+  now eapply Forall_map; cbn.
+Qed.
+
+Lemma optimize_env_wf {efl : EEnvFlags} {Σ : GlobalContextMap.t} :
+  has_tBox -> has_tRel -> 
+  wf_glob Σ -> wf_glob (optimize_env Σ).
+Proof.
+  intros hasb hasrel.
+  intros wfg. rewrite optimize_env_eq //.
+  destruct Σ as [Σ map repr wf]; cbn in *.
+  clear map repr.
+  induction wfg; cbn; constructor; auto.
+  - rewrite /= -(optimize_env_eq (GlobalContextMap.make Σ (fresh_globals_cons_inv wf))) //.
+    eapply optimize_decl_wf => //.
+  - rewrite /= -(optimize_env_eq (GlobalContextMap.make Σ (fresh_globals_cons_inv wf))) //.
+    now eapply fresh_global_optimize_env.
+Qed.
+
+Definition optimize_program (p : eprogram_env) :=
+  (EOptimizePropDiscr.optimize_env p.1, EOptimizePropDiscr.optimize p.1 p.2).
+
+Definition optimize_program_wf {efl} (p : eprogram_env) {hastbox : has_tBox} {hastrel : has_tRel} :
+  wf_eprogram_env efl p -> wf_eprogram efl (optimize_program p).
+Proof.
+  intros []; split.
+  now eapply optimize_env_wf.
+  cbn. eapply optimize_wellformed_irrel => //. now eapply optimize_wellformed.
+Qed.
+
+Definition optimize_program_expanded {efl} (p : eprogram_env) :
+  wf_eprogram_env efl p ->
+  expanded_eprogram_env_cstrs p -> expanded_eprogram_cstrs (optimize_program p).
+Proof.
+  unfold expanded_eprogram_env_cstrs.
+  move=> [wfe wft] /andP[] etae etat.
+  apply/andP; split.
+  cbn. eapply expanded_global_env_isEtaExp_env, optimize_env_expanded => //.
+  now eapply isEtaExp_env_expanded_global_env.
+  eapply expanded_isEtaExp.
+  eapply optimize_expanded_irrel => //.
+  now apply optimize_expanded, isEtaExp_expanded.
+Qed.
